

An Introduction to the Theory of Groups

Joseph J. Rotman

April 15, 2018

Fourth Edition

Problems

Chapter 1

1.13

- (i) A permutation $\alpha \in S_n$ is **regular** if either α has no fixed points and it is the product of disjoint cycles of the same length, or $\alpha = 1$. Prove that α is regular iff it is a power of an n -cycle β ; that is, $\alpha = \beta^m$ for some m . (*Hint*: if $\alpha = (a_1 a_2 \dots a_k)(b_1 b_2 \dots b_k) \dots (z_1 z_2 \dots z_k)$, where there are m letters a, b, \dots, z , then let $\beta = (a_1 b_1 \dots z_1 a_2 b_2 \dots z_2 \dots a_k b_k \dots z_k)$.)

Solution: β^m takes a_1 through $b_1 \dots z_1$ to a_2 as desired. 1 can be expressed as β^n for $\beta(j) = j + 1$ an n -cycle. For a general regular α , disjointness of the sets a_j, b_j, \dots, z_j guaranteed that the β from the hint is an n -cycle. If there's some n -cycle β with $n = mk$, and we take the m th power, we also get m disjoint, length- k cycles, as desired.

- (ii) If α is an n -cycle, then α^k is a product of $\gcd(n, k)$ disjoint cycles, each of length $n/\gcd(n, k)$.

Solution: $\alpha^n = 1$. If n is a multiple of k , then $\alpha^n = (\alpha^k)^{n/k}$. α^k would then be a product of k n/k -cycles. In the case where n is not a multiple of k , but they have a non-trivial gcd, then starting at α_0 , α would take us to α_1 . α^k will take us to α_k . It takes α_k to α_{2k} , and so on until we get to $\alpha_{mk} = \alpha_0$. This happens if $m = \frac{n}{\gcd(n, k)}$, but I don't know how to prove that.

- (iii) If p is prime, then every power of a p cycle is either a p -cycle or 1 .

Solution: This is a corollary of the last exercise, noting that $\gcd(p, k) = 1$ if $k \neq p$ and p if $k = p$.

1.17 How many $\alpha \in S_n$ are there with $\alpha^2 = 1$?

Solution: There's 1 , and there's disjoint unions of transpositions. In terms of single transpositions, there are $\binom{n}{2}$ of them. If I'm going to put together a product of j transpositions, there are $\binom{n}{2}$ ways to choose the first transposition, $\binom{n-2}{2}$ ways to choose the second, and $\binom{n-2j}{2}$ ways to choose the j th. Since any permutation of these transpositions is equivalent, I ought to get

$$1 + \sum_{j=1}^{n/2} \frac{1}{j!} \prod_{k=0}^j \binom{n-2k}{2}$$

or something, it's not important.

1.26 A group for which $x^2 = 1$ for all x must be Abelian.

Solution: We know that $aa = aea = abba = 1$, and that $abab = 1$. This implies that ab and ba must both be equal to $b^{-1}a^{-1}$.

1.27

- (i) Let G be a finite abelian group containing no elements $a \neq e$ with $a^2 = e$. Evaluate $a_1 * a_2 * \dots * a_n$, where a_1, a_2, \dots, a_n is a list of all elements in G with no repetitions.

Solution: Just for laughs, let's invert this big element. From the result of Exercise 1.23, we get $(a_1 * a_2 * \dots * a_n)^{-1} = a_n^{-1} * a_{n-1}^{-1} * \dots * a_1^{-1}$. Let A be another name for this big element, so I don't have to \LaTeX it all out. The inverses of the individual group elements are unique elements of the group themselves, so the inverse of A is another product of all elements of the group. G is abelian, so $A^{-1} = A$, since all permutations of products are equivalent. This means $A^2 = e$, and the only element of G for which that holds is 1 .

- (ii) Prove **Wilson's Theorem**: If p is prime, then

$$(p-1)! = -1 \pmod{p}.$$

(Hint: The nonzero elements of \mathbb{Z}_p form a multiplicative group.)

Solution: As far as I'm concerned, this completely contradicts the last exercise, since -1 is not the multiplicative identity unless $p = 2$. One interesting thing to note is that $(-1)^2 = 1 = 1^2$, violating the assumption of part (i). Now things start to get a little clearer. The inverse is unique, so, for all numbers from 2 up to $p-2$, the multiplicative inverse mod p is *also* in the set $\text{range}(2, p-1)$ (ranges are taken to be Python-style). That means that $(p-2)! = 1$, and $(p-1)! = p-1$, as desired.

1.31 Let G be a group, let $a \in G$, and let m and n be relatively prime integers. If $a^m = 1$, show that there exists a b such that $a = b^n$. (Hint: There are integers s and t such that $sm + tn = 1$.)

Solution: (Special thanks to Joel Klassen and Christophe Vuillot for their assistance.) We know $a^m = 1$, so that $a^{m+1} = a$. From the hint, $a^{m+sm+tn} = a$, and we can cancel multiples of m to obtain $a^{tn} = a$, so we set $b = a^t$ and get what we were after.

1.42 Let $G = \{x_1, x_2, \dots, x_n\}$ be a set equipped with an operation $*$, let $A = [a_{ij}]$ be its multiplication table (i.e. $a_{ij} = x_i * x_j$), and assume that G has a two-sided identity e : $e * x = x * e = x$ for all $x \in G$.

- (i) Show that $*$ is commutative if and only if A is symmetric.

Solution: This is true by definition.

- (ii) Show that every element $x \in G$ has a (two-sided) inverse (i.e. there is an $x' \in G$) such that $x' * x = x * x' = e$ if and only if A is a **Latin Square** (i.e. all rows and columns are permutations of G).

Solution: (Thanks to Joel Klassen and Christophe Vuillot for basically doing this problem for me). If A is a Latin Square, then there exists a left inverse and a right inverse for x , since 1 must appear in the row and column corresponding to x . $zx = 1$, $xy = 1$, therefore $zxy = z$, but $zx = 1$, so $y = z$.

Likewise, if A is not a Latin square, then there are different elements y and z such that $xy = xz = w$. If x has a left inverse, then $y = z$ and we have a contradiction. If it doesn't, we've proven what we want to prove.

- (iii) Assume that $e = x_1$ so that the first row of A has $a_{1i} = x_i$. Show that the first column of A has $a_{i1} = x_i^{-1}$ for all i if and only if $a_{ii} = 1$ for all i .

Solution: This is mad trivial.

- (iv) With the multiplication table as shown in (iii), show that $*$ is associative if and only if $a_{ij}a_{jk} = a_{ik}$.

Solution:

If: The trick here is that, if the matrix is arranged such that $\mathbb{1}$ is on the diagonal, then $a_{ij} = x_i x_j^{-1}$. If multiplication is associative, $a_{ij}a_{jk} = x_i x_j^{-1} x_j x_k^{-1} = x_i x_k^{-1} = a_{ik}$. \square

Only If: Every x_k can be expressed as $x_i x_j^{-1}$ for fixed x_i , since the multiplication table is a latin square. This implies that the product of three elements $x_k x_l x_m = x_i x_j^{-1} x_j x_n^{-1} x_n x_o^{-1} = a_{ij}a_{jn}a_{no}$. We can evaluate this product in either order, using the assumed product: $a_{ij}a_{jn}a_{no} = a_{in}a_{no} = a_{ij}a_{jo} = a_{io}$. \square

2.3 The set-theoretic union of two subgroups is a subgroup if and only if one is contained in the other. Is this true if we use three subgroups?

Solution: No, see Bruckheimer et al, 1970: <https://www.jstor.org/stable/pdf/2316854.pdf>.

2.4 Let S be a proper subgroup of G . If $G - S$ is the complement of S , prove that $\langle G - S \rangle = G$.

Solution: We know that $\langle G - S \rangle$ contains $G - S$, so all we have to prove is that the elements of S can be generated by multiplying together two things in $G - S$. Pick an element of $G - S$ g . $g^{-1} \notin S$, since that would contradict the inclusion of the inverse. Also, $sg^{-1} \notin S$ for any $s \in S$, since that would contradict closure. However, $sg^{-1} \cdot g = s$, so we can find two elements of $G - S$ that generate s under multiplication.

2.5 Let $f : G \rightarrow H$ and $g : G \rightarrow H$ be homomorphisms, and let

$$K = \{a \in G : f(a) = g(a)\}.$$

Must K be a subgroup of G ?

Solution: We need:

- the identity to be in the set. This is guaranteed by Theorem 1.13 – $f(\mathbb{1}) = \mathbb{1}'$, so $\mathbb{1} \in K$.
- closure under the inverse. This is also guaranteed by Theorem 1.13 – $f(a^{-1}) = f(a)^{-1} = g(a)^{-1} = g(a^{-1})$.
- closure under multiplication. This is guaranteed by the defining property of the homomorphism – $f(ab) = f(a)f(b) = g(a)g(b) = g(ab)$.

K is a subgroup. \square

2.7 If $n > 2$, then A_n is generated by all the 3-cycles. (*Hint:* $(ij)(jk) = (ijk)$ and $(ij)(kl) = (ijk)(jkl)$).

Solution: Parity is defined as the number of transpositions in a decomposition of a permutation. For each adjacent pair of transpositions in such a decomposition, we can apply one of the two formulae in the hint to express it as a product of 3-cycles.

2.8 Imbed S_n as a subgroup of A_{n+2} , but show that, for $n \geq 2$, S_n cannot be imbedded in A_{n+1} .

Solution: The first part is trivial. If we have elements $n + 1$ and $n + 2$, we can decide whether to multiply a permutation by $(n + 1 \ n + 2)$ on its way into the subgroup, and everything becomes even. The second part is tricky. We can easily prove that S_2 can't be imbedded in A_3 , since A_3 is generated by the 3-cycle $(1\ 2\ 3)$ which is order 3 (as are all of its subgroups), and S_2 is order 2. Jonas Helsen says that, in order to be imbedded, the order of the large group has to be an integer multiple of the order of the small group. $|S_n| = n!$ and $|A_{n+1}| = (n+1)!/2$, so the ratio is $n+1/2$, which is not an integer if n is even. We could also (try to) use the fact that, for $n + 1 \geq 5$, A_{n+1} is simple, and

S_n is not, since it has A_n as a normal subgroup. This would leave us with the $n = 3$ case, which we can allegedly show by seeing that A_4 has no subgroups of order 6. I'm not quite happy with this solution.

2.9

- (i) Prove that S_n can be generated by $\{(1\ k), k \in \mathbb{Z}_n\}$

Solution: We know that every element of S_n can be expressed as a product of transpositions, and $(j\ k) = (1\ k)(1\ j)(1\ k)$, so we're good. \square

- (ii) Prove that S_n can be generated by $\{(j\ j+1 \pmod n), j \in \mathbb{Z}_n\}$.

Solution: If we can generate the generators from the generating set in the last part, we're good. Let's use recursion, because this is *mathematics*. $(1\ k) = (1\ k-1)(k-1\ k)(1\ k-1)$.

- (iii) Prove that S_n can be generated by the two elements $(1\ 2)$ and $C = (1\ 2 \cdots n)$.

Solution: First, if I take the n th power of C , I get $\mathbb{1}$. This means that C^{-1} is the $n-1$ th power, and I can use it to generate other stuff. Let's look at $C^k(1\ 2)C^{-k}$. This operation takes $k+1 \rightarrow 1 \rightarrow 2 \rightarrow k+2$ and $k+2 \rightarrow 2 \rightarrow 1 \rightarrow k+1$, so I can generate the generators from the generating set in the last part.

- (iv) Prove that S_4 is not generated by $A = (1\ 3)$ and $C = (1\ 2\ 3\ 4)$.

Solution: I can write down an arbitrary product of these operators as $C^{i_0}AC^{i_1}AC^{i_2}\dots AC^{i_m}$. Knowing that C^{-1} is generated, I express the product as

$$C^{i_0}AC^{-i_0}C^{i_0+i_1}AC^{-(i_0+i_1)}\dots C^{\sum_{j=0}^{m-1} i_j}AC^{-\sum_{j=0}^{m-1} i_j}C^{-\sum_{j=0}^m i_j}$$

The only two values of C^iAC^{-i} are $(1\ 3)$ and $(2\ 4)$, and the only 3 non- $\mathbb{1}$ values of C^i are $(1\ 2\ 3\ 4)$, $(1\ 3)(2\ 4)$, and $(1\ 4\ 3\ 2)$. Brute force enumeration of the words of this set reveals that $(1\ 2)$ isn't generated. \square

2.12

- (i) Prove that every group G of order 4 is isomorphic either to \mathbb{Z}_4 or the 4-group \mathbf{V} .

Solution: Without loss of generality, the elements of a group of order 4 are $\mathbb{1}$, a , b , and ab . Each of these elements needs an inverse, and the inverse of the inverse is the element itself, so that if $a^{-1} = b$, then $b^{-1} = a$ also. Up to permutation of labels, there are two possible scenarios, either $a^{-1} = a$, $b^{-1} = b$, or $a^{-1} = b$. Writing out the multiplication tables then either gives us \mathbb{Z}_4 or \mathbf{V} .

- (ii) If G is a group with $|G| \leq 5$, then G is abelian.

Solution: Order 2 is trivial, there's only one non-trivial group element. 3 is prime, so the group has to be cyclic, and therefore abelian. Order 4 only permits the two groups we saw earlier, and 5 is prime.

2.16 If $H \leq G$ has index 2, then $a^2 \in H$ for every $a \in G$

Solution: (Christophe Vuillot knocked this out in 60 seconds.) If a is in H , we're done. If not, it can be expressed as gh for some h in H . Let's assume that the square is not in the subgroup. This implies $ghgh = gh'$, $\therefore hgh = h'$, $\therefore gh = h^{-1}h'$, which is a contradiction, since $h^{-1}h'$ is in H .

2.17

- (i) If $a, b \in G$ commute and if $a^m = 1 = b^n$, then $(ab)^k = 1$, where $k = \text{lcm}(m, n)$.

Solution: They commute so $(ab)^k = a^k b^k$.

- (ii) Let A and B be

$$A = \begin{bmatrix} 0 & -1 \\ 1 & 0 \end{bmatrix}, \quad B = \begin{bmatrix} 0 & 1 \\ -1 & -1 \end{bmatrix}$$

Show that $A^4 = B^3 = 1$, but AB has infinite order.

Solution: Let's take a look at the effect of AB acting from the left on a matrix.

$$\begin{bmatrix} 1 & 1 \\ 0 & 1 \end{bmatrix} \begin{bmatrix} a & b \\ c & d \end{bmatrix} = \begin{bmatrix} a+c & b+d \\ c & d \end{bmatrix}$$

This preserves c and d , so that if they were 0 and 1 on the way in, it'll be the same on the way out.

$$\begin{bmatrix} 1 & 1 \\ 0 & 1 \end{bmatrix}^k = \begin{bmatrix} 1 & k \\ 0 & 1 \end{bmatrix}$$

Note that this matrix doesn't generate the Fibonacci sequence like I thought it would, which is why I did this trivial exercise.

Note There comes a point in every yellow book where the physicist reading it will begin to skip non-trivial exercises, simply because the physicist in question is uninterested in the answers to those questions. This is that point.

2.30 If $S \leq G$ and $S = 2$, then $S \triangleleft G$.

Solution: We'd like to show that $gsg^{-1} \in S$. There are, just as in exercise 2.16, two cases. If $g \in S$, in which case $g^{-1} \in S$ and gsg^{-1} is just a product of three subgroup elements. If $g \notin S$, then $g = as_0$ with $s_0 \in S$. Let's assume that $gsg^{-1} \notin S$. This implies that $as_0ss_0^{-1}a^{-1} = as_1$, which implies $s_0ss_0^{-1}a^{-1} = s_1$. Inverting both sides, we obtain a contradiction: $as_0s^{-1}s_0^{-1}$ must be in the coset, but s_1^{-1} must be in the subgroup.

2.32 If $H \leq G$ then $H \triangleleft G$ if and only if for all $x, y \in G$, $xy \in H$ if and only if $yx \in H$.

Solution: (Solved with the assistance of Lennart Bittel) If $H \triangleleft G$ and $xy \in H$, then $gxyg^{-1} \in H$ for all g . Setting $g = x^{-1}$ gets us $yx \in H$. If $xy \in H$ implies $yx \in H$, then $xy(yx)^{-1} = xyx^{-1}y^{-1}$ is in H . This implies that, if $y^{-1} \in H$, then $xyx^{-1} \in H$ for all x . $y^{-1} \in H$ also implies $y \in H$. \square

2.38 If H and K are normal subgroups of G , show that $H \vee K \triangleleft G$.

Solution: $ghkg^{-1} = ghg^{-1}gkg^{-1} = h'k' \in H \vee K$. \square

2.39 Prove that if a normal subgroup H of G has index n , then $g^n \in H$ for all $g \in G$.

Solution: We (Christophe Vuillot and I) are going to prove that g^n is not in any coset of H , and has to, therefore, be in H . We begin by showing that, if the coset representatives are a_j for the j th coset, then $a_jh_0a_kh_1$ is not in coset j or k . Let's assume that it's in each of these cosets, and derive contradictions.

$$\begin{aligned} a_jh_0a_kh_1 &= a_jh_2 \\ h_0a_kh_1 &= h_2 \\ a_kh_1 &= h_2h_1^{-1} \end{aligned}$$

That's a contradiction, since an element in coset k can't be in the subgroup.

$$a_j h_0 a_k h_1 = a_k h_2$$

Let's use normality,

$$\begin{aligned} a_j h_0 h_1 a_k &= h_2 a_k \\ a_j h_0 h_1 &= h_2 \\ a_j h_0 &= h_2 h_1^{-1} \end{aligned}$$

Again, contradiction.

Now, let's consider g^n . $g = a_1 h$ for some a_1 in the coset representatives, and $a_1 h a_1 h$ cannot be equal to $a_1 h'$, so we say that, if it's not in H , it must be equal to some $a_2 h'$ from a separate coset. Then $g^3 = a_1 h a_1 h a_1 h$ can't be from cosets 1 or 2, g^4 can't be from cosets 1 through 3, and g^n can't be from any non- H coset.

2.41 Let G be a finite group of odd order, and let x be the product of all the elements of G in some order. Prove that $x \in G'$.

Solution: It feels like we need to use the fact that the group is odd-sized, but let's first remember that 1 is one of those elements, so the rest of the group is even-sized. Also, if $a \in G$, then $a^{-1} \in G$, so we have a randomly-arranged sequence containing each element and its inverse. I don't know what to do with this information, so let's try some small groups. Order 3 has 3 possible sequences, $aba^{-1}b^{-1}$, $aa^{-1}bb^{-1}$, $abb^{-1}a^{-1}$, two of which are the identity, and the third is a commutator. That's not too enlightening, though, so let's try one at order four. A sequence could look like $abca^{-1}b^{-1}c^{-1}$. If we're quite clever, we can write this as $a(bc)a^{-1}(cb)^{-1}$, insert the identity $a(bc)a^{-1}(bc)^{-1}(bc)(cb)^{-1}$ and expand to $a(bc)a^{-1}(bc)^{-1}bcb^{-1}c^{-1}$, and we're done.

That's sort of cool, because it doesn't depend on the size of the group. I could take some arbitrary product, find the inverse of the first element somewhere in the expression, and produce an element of the commutator group, effectively removing a variable from the expression.